heap/tree_push.v
@@ -1,0 +1,199 @@
+Require Import FloydSeq.proofauto.
+(* Require Import cprogs.heap.program. *)
+Require Import Notations Logic Datatypes.
+From Coq Require Import String List ZArith. 
+From compcert Require Import Coqlib Integers Floats AST Ctypes Cop Clight Clightdefs.
+Require Import Coq.Logic.Classical_Pred_Type.
+Require Import Coq.Logic.Classical_Prop.
+
+Require Import Coq.micromega.Psatz.
+Local Open Scope string.
+Local Open Scope nat_scope.
+Local Open Scope Z_scope.
+Local Open Scope list_scope.
+Require Import cprogs.heap.list_relation.
+Require Import cprogs.heap.definitions.
+Require Import cprogs.heap.tree_list.
+
+Require Import SetsClass.SetsClass.
+Local Open Scope sets.
+Import SetsNotation.
+
+Inductive list_nth_on_partial_tree (l: list Z) (n: Z) (p: Z) (lt: partial_tree) : Prop :=
+  | nth_partial_tree_nil: p = n -> lt = nil -> list_nth_on_partial_tree l n p lt
+  | nth_partial_tree_cons: forall flg v t lt0, 
+    lt = (flg, v, t) :: lt0 ->
+    1 <= (p / 2) < Zlength l -> 
+    p = (p / 2) * 2 + (if flg then 1 else 0) ->
+    Znth (p / 2) l = v -> 
+    list_nth_on_tree l (p + (if flg then -1 else 1)) t -> 
+    list_nth_on_partial_tree l n (p / 2) lt0 -> 
+    list_nth_on_partial_tree l n p lt.
+
+
+Lemma list_nth_on_partial_tree_app: forall l n p lt (flg: bool) v t,
+  (if flg then
+    list_nth_on_partial_tree l (n * 2 + 1) p lt /\ list_nth_on_tree l (n * 2) t /\ Znth n l = v
+  else
+    list_nth_on_partial_tree l (n * 2) p lt /\ list_nth_on_tree l (n * 2 + 1) t /\ Znth n l = v) ->
+  1 <= n < Zlength l ->
+  list_nth_on_partial_tree l n p (lt ++ [(flg, v, t)]).
+Proof.
+  intros.
+  destruct flg.
+  {
+    revert l p v n t H H0.
+    induction lt; intros; simpl; destruct H as [? [? ?] ].
+    + inversion H; [ | discriminate].
+      pose proof Z.div_lt_upper_bound p 2 (n + 1) ltac:(lia) ltac:(lia).
+      pose proof Z.div_le_lower_bound p 2 n ltac:(lia) ltac:(lia).
+      eapply nth_partial_tree_cons; eauto; simpl.
+      * inversion H; [lia | discriminate].
+      * lia. 
+      * replace (p / 2) with n by lia; tauto.
+      * replace (p + -1) with (n * 2) by lia; tauto.
+      * apply nth_partial_tree_nil; [lia | tauto].
+    + destruct a as [[flga va] ta].
+      inversion H; [discriminate | ].
+      injection H3; intros; subst lt0 ta va flga.
+      eapply nth_partial_tree_cons; eauto.
+  }
+  {
+    revert l p v n t H H0.
+    induction lt; intros; simpl; destruct H as [? [? ?] ].
+    + inversion H; [ | discriminate].
+      pose proof Z.div_lt_upper_bound p 2 (n + 1) ltac:(lia) ltac:(lia).
+      pose proof Z.div_le_lower_bound p 2 n ltac:(lia) ltac:(lia).
+      eapply nth_partial_tree_cons; eauto; simpl.
+      * inversion H; [lia | discriminate].
+      * lia. 
+      * replace (p / 2) with n by lia; tauto.
+      * replace (p + 1) with (n * 2 + 1) by lia; tauto.
+      * apply nth_partial_tree_nil; [lia | tauto].
+    + destruct a as [[flga va] ta].
+      inversion H; [discriminate | ].
+      injection H3; intros; subst lt0 ta va flga.
+      eapply nth_partial_tree_cons; eauto.
+  }
+Qed.
+
+Fixpoint tree_next_log (d: Z) (tr: tree): Z :=
+  match tr with
+  | Leaf => 1
+  | Node v ls rs => 
+    if full_tree_b (d - 2) rs then
+      2 * tree_next_log (d - 1) ls
+    else
+      2 * tree_next_log (d - 1) rs
+  end.
+
+Lemma next_index_lowbit: forall n d t,
+  complete_tree_push d t ->
+  next_index d n t = n * (tree_next_log d t) + next_index d 0 t.
+Proof.
+  intros.
+  revert d n H.
+  induction t; simpl; intros.
+  + lia.
+  + inversion H; subst v t1 t2.
+    - assert (full_tree_b (d - 1) ls = true) by admit.
+      rewrite H0; simpl.   
+      specialize (IHt2 (d - 1)).
+      remember IHt2 as IHt2'; clear HeqIHt2'.
+      specialize (IHt2' 1 H4).
+      rewrite IHt2'.
+      specialize (IHt2 (n * 2 + 1) H4).
+      rewrite IHt2.
+      lia. 
+    - assert (full_tree_b (d - 2) rs = true) by admit.
+      rewrite H0; simpl.   
+      specialize (IHt1 (d - 1) (n * 2) H2).
+      rewrite IHt1.
+      lia. 
+Admitted.
+  
+Lemma complete_tree_next_index: forall d t,
+  complete_tree_push d t ->
+  next_index d 1 t = tree_size t + 1.
+Proof.
+  intros.
+  revert d H.
+  induction t; simpl; intros.
+  2: {
+    inversion H; subst v t1 t2.
+    + assert (full_tree_b (d - 2) rs = false) by admit.
+      rewrite H0; simpl.
+      specialize (IHt2 (d - 1) H4).
+      rewrite IHt2.
+      lia.  
+  }  
+Qed.
+
+Lemma list_on_tree_decompose: forall l n d t,
+  list_nth_on_tree l n t ->
+  complete_tree_push d t ->
+  exists pt, t = tree_compose pt Leaf /\
+  list_nth_on_partial_tree l n (next_index d n t) pt.
+Proof.
+  intros.
+  revert n H.
+  induction H0; intros.
+  + exists nil.
+    split; auto.
+    constructor; auto.
+  + inversion H1; subst v0 ls0 rs0.
+    specialize (IHcomplete_tree_push _ H8).
+    destruct IHcomplete_tree_push as [pt [? ?] ].
+    exists (pt ++ [(true, v, ls)]).
+    split.
+    - rewrite tree_compose_append.
+      rewrite H2.
+      auto.
+    - apply list_nth_on_partial_tree_app; [ | lia].
+      split; [ | split].
+      * simpl.
+        assert (full_tree_b (dep - 2) rs = false) by admit.
+        rewrite H4; tauto.
+      * tauto.
+      * tauto.
+  + inversion H1; subst v0 ls0 rs0.
+    specialize (IHcomplete_tree_push _ H7).
+    destruct IHcomplete_tree_push as [pt [? ?] ].
+    exists (pt ++ [(false, v, rs)]).
+    split.
+    - rewrite tree_compose_append.
+      rewrite H2.
+      auto.
+    - apply list_nth_on_partial_tree_app; [ | lia].
+      split; [ | split].
+      * simpl.
+        assert (full_tree_b (dep - 2) rs = true) by admit.
+        rewrite H4; tauto.
+      * tauto.
+      * tauto. 
+Admitted.
+
+Lemma list_on_tree_state_app: forall (l: list Z) (t: tree) (v: Z),
+  Zlength l >= 1 -> list_on_tree l t -> 
+  exists pt, list_on_tree_state (l++[v], Zlength l) (pt, Node v Leaf Leaf).
+Proof.
+  intros.
+  unfold list_on_tree in H0.
+  destruct H0 as [? [? [d ?]]].
+  unfold list_on_tree_state; simpl.
+  unfold list_on_tree_state_fix.
+  pose proof tree_push_decompose_sound _ _ v H2.
+  destruct H3 as [pt [? ?] ].
+  exists pt.
+  split.
+  + apply list_nth_on_tree_Node.
+    - rewrite Zlength_app.
+      replace (Zlength [v]) with 1 by auto.
+      lia.
+    - rewrite app_Znth2 by lia.
+      replace (Zlength l - Zlength l) with 0 by lia.
+      auto.
+    - constructor.
+    - constructor.
+  +      
+Qed.
